examples/logic/ltl/relationTheoryHelperScript.sml
@@ -8,4 +8,22 @@ val RTC_TRANSITIVE = store_thm
    metis_tac[RTC_TRANSITIVE,transitive_def]
   );
 
+val REFL_THM = store_thm
+  ("REFL_THM",
+   ``!R. reflexive R = !x y. R x x``,
+   fs[reflexive_def]
+  );
+
+val TRANS_THM = store_thm
+  ("TRANS_THM",
+   ``!R. transitive R = !x y z. R x y ∧ R y z ==> R x z``,
+   fs[transitive_def]
+  );
+
+val SYMM_THM = store_thm
+  ("SYMM_THM",
+   ``!R. symmetric R = (!x y. R x y =  R y x)``,
+    fs[symmetric_def]
+  );
+
 val _ = export_theory();
